In~\cite{gregory2023iterated}, Gregory et al.
provide the following conjecture for row sums of iterated rascal triangles.
\begin{conjecture}
    \label{conjecture:row_sums}
    For every $i$
    \begin{align*}
        \sum_{k=0}^{4i+3} \rascalNumber{4i+3}{k}{i} = 2^{4i+2}
    \end{align*}
\end{conjecture}
where $\rascalNumber{n}{k}{i}$ is an iterated rascal number.
Define the iterated rascal number
\begin{definition}
    Iterated rascal number
    \begin{align*}
        \rascalNumber{n}{k}{i} &= \sum_{m=0}^{i} \binom{n-k}{m} \binom{k}{m}
    \end{align*}
\end{definition}
Note that iterated rascal numbers are closely related to Vandermonde convolution
$\binom{a+b}{r} = \sum_{m=0}^{r} \binom{a}{m} \binom{b}{r-m}$
\begin{equation*}
    \rascalNumber{n}{k}{i} = \sum_{m=0}^{i} \binom{n-k}{m} \binom{k}{k-m}
\end{equation*}
While
\begin{equation*}
    \binom{n}{k}= \sum_{m=0}^{k} \binom{n-k}{m} \binom{k}{k-m}
\end{equation*}
It is straightforward to see that
\begin{equation*}
    \binom{n}{k} - \rascalNumber{n}{k}{i} = \sum_{m=i+1}^{k} \binom{n-k}{m} \binom{k}{k-m}
\end{equation*}
In particular, above sum is zero for $k \leq i$, that means
\begin{equation*}
    \binom{n}{k} = \rascalNumber{n}{k}{i}, \quad  0 \leq k \leq i
\end{equation*}
To prove the conjecture~\eqref{conjecture:row_sums}
we utilize above relations in terms of binomial coefficients and iterated rascal numbers.
Recall the row sums property of binomial coefficients
\begin{equation*}
    \sum_{k=0}^{4i+3} \binom{4i+3}{k} = 2^{4i+3}
\end{equation*}
If conjecture~\eqref{conjecture:row_sums} is true, then it is also true that
\begin{equation*}
     \sum_{k=0}^{4i+3} \binom{4i+3}{k} -  \sum_{k=0}^{4i+3} \binom{4i+3}{k}_i = 2^{4i+2}
\end{equation*}
because $2^{4i+3} - 2^{4i+2} = 2^{4i+2}$.
Expanding both sums we get
\begin{align*}
    2^{4i+2} &= \sum_{k=0}^{4i+3} \sum_{m=0}^{k} \binom{4i+3-k}{m} \binom{k}{k-m} - \sum_{k=0}^{4i+3} \sum_{m=0}^{i} \binom{4i+3-k}{m} \binom{k}{k-m}\\
    2^{4i+2} &= \sum_{k=0}^{4i+3} \sum_{m=0}^{k} \binom{4i+3-k}{m} \binom{k}{k-m} - \sum_{m=0}^{i} \binom{4i+3-k}{m} \binom{k}{k-m}
\end{align*}
Note that $\binom{n}{k} \geq \binom{n}{k}_i$ for each $n,k,i$.
Now we have three possible relation between $i,k$: $k < i$, $k = i$, $k > i$.

If $k < i$ then inner sums turn into
\begin{equation*}
    \sum_{m=0}^{k} \binom{4i+3-k}{m} \binom{k}{k-m} - \sum_{m=0}^{i} \binom{4i+3-k}{m} \binom{k}{k-m}
    = - \sum_{m=k}^{i} \binom{4i+3-k}{m} \binom{k}{k-m}
\end{equation*}
If $k = i$ obviously
\begin{equation*}
    \sum_{m=0}^{k} \binom{4i+3-k}{m} \binom{k}{k-m} - \sum_{m=0}^{i} \binom{4i+3-k}{m} \binom{k}{k-m} = 0
\end{equation*}
If $k > i$ then
\begin{equation*}
    \sum_{m=0}^{k} \binom{4i+3-k}{m} \binom{k}{k-m} - \sum_{m=0}^{i} \binom{4i+3-k}{m} \binom{k}{k-m}
    = \sum_{m=i}^{k} \binom{4i+3-k}{m} \binom{k}{k-m}
\end{equation*}
